Weidenbach_Book/IsaSAT_Watch_List_LLVM.thy
@@ -1,0 +1,10 @@
+theory IsaSAT_Watch_List_LLVM
+  imports IsaSAT_Watch_List IsaSAT_Literals_LLVM
+begin
+
+type_synonym watched_wl_uint32 
+  = \<open>(32,(64 word \<times> 32 word \<times> 1 word),64)array_array_list\<close>
+
+abbreviation "watcher_fast_assn \<equiv> uint64_nat_assn *a unat_lit_assn *a bool1_assn   "
+
+end
